A first try with existing modifies clauses

test/LinkedList1.fst
@@ -31,17 +31,18 @@ and cell (a: Type0) =
 /// - the absence of cycles does not suffice to guarantee termination, as the
 ///   number of references in the heap is potentially infinite;
 /// - the heap model allows us to select without showing liveness, which allows
-///   to de-couple the length predicate from the liveness predicate.
-let rec list_has_length #a (h: HS.mem) (c: t a) (l: nat):
-  GTot bool (decreases l)
-=
-  match HS.sel h c with
-  | Nil -> l = 0
-  | Cons next _ ->
+///   to de-couple the length predicate from the liveness predicate. (YES, it allows us to, but it deserves nothing. )
+let rec well_formed #a (h: HS.mem) (c: t a) (l: nat):
+  GTot Type0 (decreases l)
+= HS.contains h c /\ (
+    match HS.sel h c with
+    | Nil -> l = 0
+    | Cons next _ ->
       if l = 0 then
         false
       else
-        list_has_length h next (l - 1)
+        well_formed h next (l - 1)
+  )
 
 /// Note: all the ghost predicates and functions operate on a length of type
 /// nat; the Ghost effect guarantees that the length can only be used at
@@ -50,63 +51,28 @@ let rec list_has_length #a (h: HS.mem) (c: t a) (l: nat):
 /// computationally-irrelevant and can be safely removed from the resulting C
 /// code via a combination of F* + KreMLin erasure.
 
-/// When traversing a list `l` such that `list_has_length h l n`, it is often
+/// When traversing a list `l` such that `well_formed h l n`, it is often
 /// the case that we recursively visit the Cons cell, passing `n - 1` for the
 /// recursive call. This lemma ensures that Z3 can show that `n - 1` has type
 /// `nat`.
 let cons_nonzero_length #a (h: HS.mem) (c: ref (cell a)) (l: nat):
   Lemma
-    (requires (list_has_length h c l /\ Cons? (HS.sel h c)))
+    (requires (well_formed h c l /\ Cons? (HS.sel h c)))
     (ensures (l <> 0))
-    [ SMTPat (list_has_length h c l); SMTPat (Cons? (HS.sel h c)) ] =
+    [ SMTPat (well_formed h c l); SMTPat (Cons? (HS.sel h c)) ] =
     ()
 
-/// The contraposition of this lemma allows deriving that if two lengths are
-/// different, then the corresponding references are disjoint.
-let rec length_injective #a (h: HS.mem) (c: ref (cell a)) (l1 l2: nat):
+let rec length_functional #a (h: HS.mem) (c: ref (cell a)) (l1 l2: nat):
   Lemma
-    (requires (list_has_length h c l1 /\ list_has_length h c l2))
+    (requires (well_formed h c l1 /\ well_formed h c l2))
     (ensures (l1 = l2))
     (decreases l1)
-    [ SMTPat (list_has_length h c l1); SMTPat (list_has_length h c l2) ] =
+    [ SMTPat (well_formed h c l1); SMTPat (well_formed h c l2) ] =
   match HS.sel h c with
   | Nil -> ()
   | Cons next _ ->
       // Without `cons_nonzero_length`, we would need assert (l1 <> 0)
-      length_injective h next (l1 - 1) (l2 - 1)
-
-/// For this example, we let all references live in the general region of the
-/// heap. The `contains` predicate is needed by several lemmas from the heap
-/// library, so we list it here.
-///
-/// The liveness predicate is `contains`: as an approximation, the underlying
-/// heap model represents each region as a map from addresses to their values,
-/// and contains asserts that the reference is in the domain of the map.
-///
-/// TODO: figure out why the predicate is called contains instead of
-/// TODO: figure out why we need frameOf
-let cell_is_live #a (h: HS.mem) (c: t a) =
-  HS.frameOf c = HS.root /\
-  HS.contains h c
-
-/// This predicate states that all the cells are live. It relies on
-/// `list_has_length` for its termination.
-/// TODO: figure out why `cell_is_live h l /\ (match ...)` doesn't work.
-let rec list_is_live #a #n (h: HS.mem) (l: t a {list_has_length h l n}):
-  Tot Type (decreases n)
-=
-  match HS.sel h l with
-  | Nil ->
-      cell_is_live h l /\
-      True
-  | Cons next _ ->
-      cell_is_live h l /\
-      list_is_live #a #(n - 1) h next
-
-/// Thus, a well-formed list is both paired with a predicate for its length, and
-/// states that are the list cells are live in the current heap.
-let well_formed #a (h: HS.mem) (l: t a) (n: nat) =
-  list_has_length h l n /\ list_is_live #a #n h l
+      length_functional h next (l1 - 1) (l2 - 1)
 
 /// This form will rarely turn out to be useful, except perhaps for user code.
 /// Indeed, we most often want to tie the length of the list in the final state
@@ -114,68 +80,139 @@ let well_formed #a (h: HS.mem) (l: t a) (n: nat) =
 let live #a (h: HS.mem) (l: t a) =
   exists n. well_formed #a h l n
 
+let live_nil #a (h: HS.mem) (l: ref (cell a)) : Lemma
+  (requires (HS.contains h l /\ Nil? (HS.sel h l)))
+  (ensures (live h l))
+= assert (well_formed h l 0)
+
+let live_cons #a (h: HS.mem) (l: ref (cell a)) : Lemma
+  (requires (HS.contains h l /\ Cons? (HS.sel h l) /\ live h (Cons?.next (HS.sel h l))))
+  (ensures (live h l))
+= assert (forall n . well_formed h (Cons?.next (HS.sel h l)) n ==> well_formed h l (n + 1))
+
+/// TODO: move to FStar.Monotonic.HyperStack
+/// Disjointness of two references
+
+let disjoint (#a1 #a2: Type) (r1: ref a1) (r2: ref a2) : GTot bool =
+  HS.frameOf r1 <> HS.frameOf r2 || HS.as_addr r1 <> HS.as_addr r2
+
+/// Disjointness of a reference wrt. a list of references of the same type
+
+let rec disjoint_from_list (#a #b: Type) (r: ref a) (l: list (ref b)) : GTot bool =
+  match l with
+  | [] -> true
+  | r' :: q -> disjoint r r' && disjoint_from_list r q
 
 /// As we start proving some degree of functional correctness, we will have to
 /// reason about non-interference, and state that some operations do not modify
 /// the footprint of a given list.
 /// TODO: there's a non-replayable hint here
-#set-options "--max_ifuel 0 --max_fuel 1"
+#set-options "--max_ifuel 1 --max_fuel 2"
 val footprint: (#a: Type) -> (h: HS.mem) -> (l: t a) -> (n: nat) -> Ghost (list (ref (cell a)))
   (requires (well_formed h l n))
   (ensures (fun refs ->
     let n_refs = L.length refs in
-    n_refs = n /\
+    n_refs == n + 1 /\
     (forall (i: nat). {:pattern (L.index refs i)}
-      i < n ==> well_formed h (L.index refs i) (n - i))))
+      i <= n ==> well_formed h (L.index refs i) (n - i))))
   (decreases n)
 
 let rec footprint #a h l n =
   match HS.sel h l with
   | Nil ->
-      []
+      [l]
   | Cons next _ ->
       let refs = footprint h next (n - 1) in
       l :: refs
 #reset-options
 
-/// There are several views of references; by default, references do not support
-/// decidable equality, i.e. the heap model does not expose pointer comparisons.
-/// One can, however, reason about equality of addresses (ghostly, i.e. in
-/// proofs only) by using `HS.as_addr`. From two references having distinct
-/// addresses, it follows that writing to one leaves the other untouched.
-
-/// All the reasoning about the pop operation is done in this lemma. If `head`
-/// is not found in the footprint of `l`, then the specific write we perform for
-/// pop (we could be more generic!) leaves the two essential predicates
-/// untouched for l.
-/// TODO: this proof is slow / investigate
-
-val pop_preserves_live: (#a: Type) -> (h0: HS.mem) -> (head: ref (cell a)) -> (l: t a) -> (n: nat) ->
-  Lemma
-    (requires (
-      live h0 head /\
-      Cons? (HS.sel h0 head) /\
-      well_formed h0 l n /\ (
-      let refs = footprint h0 l n in
-      forall (i: nat). // {:pattern well_formed h0 (L.index refs i) (n - i)}
-        i < n ==> HS.as_addr head <> HS.as_addr (L.index refs i))
-    ))
-    (ensures (
-      live h0 head /\
-      Cons? (HS.sel h0 head) /\ (
-      let next = Cons?.next (HS.sel h0 head) in
-      let h1 = HS.upd h0 head (HS.sel h0 next) in
-      well_formed h1 l n)
-    ))
-    (decreases n)
-    [ SMTPat (well_formed #a h0 l n); SMTPat (Cons? (HS.sel h0 head)) ]
-
-#set-options "--z3rlimit 40 --max_ifuel 0"
-let rec pop_preserves_live #a h0 head l n =
-  match HS.sel h0 l with
+let rec modifies_disjoint_footprint
+  (#a: Type)
+  (#b: Type)
+  (h: HS.mem)
+  (l: t a)
+  (n: nat)
+  (r: ref b)
+  (h' : HS.mem)
+: Lemma
+  (requires (
+    well_formed h l n /\
+    disjoint_from_list r (footprint h l n) /\
+    HS.modifies_one (HS.frameOf r) h h' /\
+    HS.modifies_ref (HS.frameOf r) (Set.singleton (HS.as_addr r)) h h'
+  ))
+  (ensures (
+    well_formed h' l n /\
+    footprint h' l n == footprint h l n
+  ))
+  (decreases n)
+= match HS.sel h l with
   | Nil -> ()
-  | Cons l' _ ->
-      pop_preserves_live h0 head l' (n - 1)
+  | Cons l' _ -> modifies_disjoint_footprint h l' (n - 1) r h'
+
+let rec well_formed_distinct_lengths_disjoint
+  #a1 #a2
+  (c1: ref (cell a1))
+  (c2: ref (cell a2))
+  (n1: nat)
+  (n2: nat)
+  (h: HS.mem)
+: Lemma
+  (requires (
+    well_formed h c1 n1 /\
+    well_formed h c2 n2 /\
+    n1 <> n2
+  ))
+  (ensures (
+    disjoint c1 c2
+  ))
+  (decreases (n1 + n2))
+= match HS.sel h c1, HS.sel h c2 with
+  | Cons next1 _, Cons next2 _ ->
+    well_formed_distinct_lengths_disjoint next1 next2 (n1 - 1) (n2 - 1) h
+  | _ -> ()
+
+let rec well_formed_gt_lengths_disjoint_from_list
+  #a1 #a2
+  (h: HS.mem)
+  (c1: ref (cell a1))
+  (c2: ref (cell a2))
+  (n1: nat)
+  (n2: nat)
+: Lemma
+  (requires (well_formed h c1 n1 /\ well_formed h c2 n2 /\ n1 > n2))
+  (ensures (disjoint_from_list c1 (footprint h c2 n2)))
+  (decreases n2)
+= well_formed_distinct_lengths_disjoint c1 c2 n1 n2 h;
+  if n2 = 0
+  then ()
+  else well_formed_gt_lengths_disjoint_from_list h c1 (Cons?.next (HS.sel h c2)) n1 (n2 - 1)
+
+let well_formed_head_tail_disjoint
+  #a
+  (h: HS.mem)
+  (c: ref (cell a))
+  (n: nat)
+: Lemma
+  (requires (well_formed h c n))
+  (ensures (let (hd :: tl) = footprint h c n in hd == c /\ disjoint_from_list c tl))
+= if n = 0
+  then ()
+  else well_formed_gt_lengths_disjoint_from_list h c (Cons?.next (HS.sel h c)) n (n - 1)
+
+let rec unused_in_well_formed_disjoint_from_list
+  #a #b
+  (h: HS.mem)
+  (r: ref a)
+  (l: ref (cell b))
+  (n: nat)
+: Lemma
+  (requires (r `HS.unused_in` h /\ well_formed h l n))
+  (ensures (disjoint_from_list r (footprint h l n)))
+  (decreases n)
+= if n = 0
+  then ()
+  else unused_in_well_formed_disjoint_from_list h r (Cons?.next (HS.sel h l)) (n - 1)
 
 /// Finally, the pop operation. Our representation of linked lists is slightly
 /// unusual, owing to the fact that we do not have null references, and
@@ -209,7 +246,9 @@ let pop #a #n l =
   | Cons next data ->
       let h0 = get () in
       l := !next;
-      pop_preserves_live #a h0 l next (G.reveal n - 1);
+      let h1 = get () in
+      well_formed_head_tail_disjoint h0 l (G.reveal n);
+      modifies_disjoint_footprint h0 next (G.reveal n - 1) l h1;
       Some data
 
 val push: (#a: Type) -> (#n: G.erased nat) -> (l: t a) -> (x: a) ->
@@ -218,14 +257,18 @@ val push: (#a: Type) -> (#n: G.erased nat) -> (l: t a) -> (x: a) ->
     (ensures (fun h0 () h1 -> well_formed h1 l (G.reveal n + 1)))
 
 let push #a #n l x =
+  let h0 = get () in
   let c: ref (cell a) = ralloc HS.root !l in
-  // need to write a lemma that states that allocation preserves the live
-  // predicate for lists
+  unused_in_well_formed_disjoint_from_list h0 c l (G.reveal n);
+  let h1 = get () in
+  modifies_disjoint_footprint h0 l (G.reveal n) c h1;
   l := Cons c x;
-  admit ()
+  let h2 = get () in
+  well_formed_head_tail_disjoint h0 l (G.reveal n);
+  modifies_disjoint_footprint h1 c (G.reveal n) l h2
 
 
-/// Connecting our predicate `list_has_length` to the regular length function.
+/// Connecting our predicate `well_formed` to the regular length function.
 /// Note that this function takes a list whose length is unknown statically,
 /// because of the existential quantification.
 /// TODO: figure out why the `assert` is needed.
@@ -245,7 +288,7 @@ let rec length #a gn l =
   match !l with
   | Nil ->
       let h = get () in
-      assert (list_has_length h l 0);
+      assert (well_formed h l 0);
       0ul
   | Cons next _ ->
       let open U32 in
